io/MIO.Sig.Call.fst
@@ -2,6 +2,8 @@ module MIO.Sig.Call
 
 open MIO.Sig
 
+assume val print_string2 : string -> Tot bool
+
 (** This file is replaced during linking with a file that contains the real
 implementation of the commands. **)
 let mio_call (caller:bool) (cmd:cmds) (arg:mio_sig.args cmd) : mio (mio_sig.res cmd arg) =
