io/case-study/GoodHandler2.fst
@@ -15,7 +15,12 @@ type tgt_handler = ctx_tgt tgt_cs_int
 
 val good_handler2 : tgt_handler
 let good_handler2 #fl io_acts client req send =
-  send req
+  let r = send req in
+  let x = (let x = MIO.Sig.Call.print_string2 "Returning result from request handler..." in
+  match r, x with
+  | Inl (), _ -> MIO.Sig.Call.print_string2 "(Inl ())\n"
+  | Inr _, _ -> MIO.Sig.Call.print_string2 "(Inr _)\n") in
+  fst (r,x)
 
 let good_main2 : comp.target.whole = comp.target.link compiled_webserver good_handler2
 
